Continue updating data_to_wordProps
Including with help from Magnus.
The tagging scheme seems workable.

Changed the representation of byte arrays slightly (the last word needs
to be zeroed out beyond the last byte) so we can reuse the word_cmp_loop
test when comparing byte arrays (which compares a whole word a at a
time).

There is cheat in word_eq_thm about using word_cmp_loop. And the
compiler needs to be changed for RefByte.

(issue #100)

compiler/backend/proofs/data_to_wordPropsScript.sml
@@ -11,6 +11,12 @@ val _ = new_theory "data_to_wordProps";
 val clean_tac = rpt var_eq_tac \\ rpt (qpat_x_assum `T` kall_tac)
 fun rpt_drule th = drule (th |> GEN_ALL) \\ rpt (disch_then drule \\ fs [])
 
+val _ = augment_srw_ss[rewrites[LENGTH_REPLICATE]]
+
+val LESS_4 = DECIDE ``i < 4 <=> (i = 0) \/ (i = 1) \/ (i = 2) \/ (i = 3n)``
+val LESS_8 = DECIDE ``i < 8 <=> (i = 0) \/ (i = 1) \/ (i = 2) \/ (i = 3n) \/
+                                (i = 4) \/ (i = 5) \/ (i = 6) \/ (i = 7)``
+
 val word_bit_thm = store_thm("word_bit_thm",
   ``!n w:'a word. word_bit n w <=> n < dimindex (:'a) /\ w ' n``,
   fs [word_bit_def,LESS_EQ] \\ rw []
@@ -247,9 +253,9 @@ val bc_ref_inv_def = Define `
         (?zs. (heap_lookup x heap = SOME (RefBlock zs)) /\
               EVERY2 (\z y. v_inv conf y (z,f,heap)) zs ys)
     | (SOME x, SOME (ByteArray flag bs)) =>
-        ?ws. LENGTH bs ≤ LENGTH ws * (dimindex (:α) DIV 8) /\
-             LENGTH ws ≤ LENGTH bs DIV (dimindex (:α) DIV 8) + 1 /\
-             (heap_lookup x heap = SOME (Bytes be flag bs (ws:'a word list)))
+        ?ws. LENGTH bs ≤ ws * (dimindex (:α) DIV 8) /\
+             ws ≤ LENGTH bs DIV (dimindex (:α) DIV 8) + 1 /\
+            (heap_lookup x heap = SOME (Bytes be flag bs (REPLICATE ws (0w:'a word))))
     | _ => F`;
 
 val bc_stack_ref_inv_def = Define `
@@ -1637,10 +1643,10 @@ val update_byte_ref_thm = Q.store_thm("update_byte_ref_thm",
   \\ fs [FLOOKUP_DEF] \\ rw []
   \\ drule heap_lookup_SPLIT \\ rw [] \\ fs []
   \\ qexists_tac `ha` \\ fs []
-  \\ qexists_tac `ws` \\ fs [PULL_EXISTS]
+  \\ qexists_tac `REPLICATE ws 0w` \\ fs [PULL_EXISTS]
   \\ qexists_tac `f` \\ fs []
-  \\ `!a. isSomeDataElement (heap_lookup a (ha ++ [Bytes be fl ys ws] ++ hb)) =
-          isSomeDataElement (heap_lookup a (ha ++ [Bytes be fl xs ws] ++ hb))` by
+  \\ `!a. isSomeDataElement (heap_lookup a (ha ++ [Bytes be fl ys (REPLICATE ws 0w)] ++ hb)) =
+          isSomeDataElement (heap_lookup a (ha ++ [Bytes be fl xs (REPLICATE ws 0w)] ++ hb))` by
    (rw [] \\ fs [isSomeDataElement_def] \\ rw []
     \\ fs [heap_lookup_APPEND] \\ rw [] \\ rw [] \\ fs []
     \\ fs [heap_length_def,Bytes_def,el_length_def,heap_lookup_def])
@@ -1911,19 +1917,19 @@ val el_thm = Q.store_thm("el_thm",
 
 val new_byte_thm = Q.store_thm("new_byte_thm",
   `abs_ml_inv conf stack refs (roots,heap,be,a,sp) limit /\
-    LENGTH bs ≤ LENGTH (ws:'a word list) * (dimindex (:α) DIV 8) ∧
-    LENGTH ws ≤ LENGTH bs DIV (dimindex (:α) DIV 8) + 1 /\
-    ~(ptr IN FDOM refs) /\ LENGTH ws + 1 <= sp ==>
+    LENGTH bs ≤ ws * (dimindex (:α) DIV 8) ∧
+    ws ≤ LENGTH bs DIV (dimindex (:α) DIV 8) + 1 /\
+    ~(ptr IN FDOM refs) /\ ws + 1 <= sp ==>
     ?heap2.
-      (heap_store_unused a sp (Bytes be fl bs (ws:'a word list)) heap = (heap2,T)) /\
+      (heap_store_unused a sp (Bytes be fl bs (REPLICATE ws (0w:'a word))) heap = (heap2,T)) /\
       abs_ml_inv conf ((RefPtr ptr)::stack) (refs |+ (ptr,ByteArray fl bs))
-                 (Pointer (a+sp-(LENGTH ws + 1)) (Word 0w)::roots,heap2,be,a,
-                  sp - (LENGTH ws + 1)) limit`,
+                 (Pointer (a+sp-(ws + 1)) (Word 0w)::roots,heap2,be,a,
+                  sp - (ws + 1)) limit`,
   simp_tac std_ss [abs_ml_inv_def]
   \\ rpt strip_tac \\ full_simp_tac std_ss [bc_stack_ref_inv_def]
   \\ imp_res_tac EVERY2_APPEND_IMP_APPEND
   \\ full_simp_tac (srw_ss()) []
-  \\ `el_length (Bytes be fl bs ws) <= sp` by ALL_TAC
+  \\ `el_length (Bytes be fl bs (REPLICATE ws 0w)) <= sp` by ALL_TAC
   THEN1 (fs [el_length_def,Bytes_def])
   \\ qpat_x_assum `unused_space_inv a sp heap` (fn th =>
     MATCH_MP (IMP_heap_store_unused
@@ -1940,18 +1946,18 @@ val new_byte_thm = Q.store_thm("new_byte_thm",
    (fs [heap_ok_def,Bytes_def,isForwardPointer_def] \\ rveq \\ rw []
     \\ res_tac \\ full_simp_tac std_ss [heap_store_rel_def]
     \\ POP_ASSUM MP_TAC \\ full_simp_tac (srw_ss()) [])
-  \\ `unused_space_inv a (sp - (LENGTH ws + 1)) heap2` by ALL_TAC
+  \\ `unused_space_inv a (sp - (ws + 1)) heap2` by ALL_TAC
   THEN1 fs [Bytes_def,el_length_def] \\ fs []
   \\ `~(ptr IN FDOM f)` by (full_simp_tac (srw_ss()) [SUBSET_DEF] \\ metis_tac [])
-  \\ qexists_tac `f |+ (ptr,a+sp-(LENGTH ws + 1))`
+  \\ qexists_tac `f |+ (ptr,a+sp-(ws + 1))`
   \\ strip_tac THEN1
    (full_simp_tac (srw_ss()) [FDOM_FUPDATE]
-    \\ `(FAPPLY (f |+ (ptr,a + sp - (LENGTH ws + 1)))) =
-          (ptr =+ (a+sp-(LENGTH ws + 1))) (FAPPLY f)` by
+    \\ `(FAPPLY (f |+ (ptr,a + sp - (ws + 1)))) =
+          (ptr =+ (a+sp-(ws + 1))) (FAPPLY f)` by
      (full_simp_tac std_ss [FUN_EQ_THM,FAPPLY_FUPDATE_THM,APPLY_UPDATE_THM]
       \\ metis_tac []) \\ full_simp_tac std_ss []
     \\ match_mp_tac (METIS_PROVE [] ``!y. (x = y) /\ f y ==> f x``)
-    \\ qexists_tac `(a + sp - (LENGTH ws + 1)) INSERT
+    \\ qexists_tac `(a + sp - (ws + 1)) INSERT
          {a | isSomeDataElement (heap_lookup a heap)}`
     \\ strip_tac
     THEN1 (fs [Bytes_def,LET_DEF,isDataElement_def,el_length_def])
@@ -1961,7 +1967,7 @@ val new_byte_thm = Q.store_thm("new_byte_thm",
     \\ fs [isDataElement_def])
   \\ strip_tac THEN1
      (full_simp_tac (srw_ss()) [SUBSET_DEF,FDOM_FUPDATE] \\ metis_tac [])
-  \\ Q.ABBREV_TAC `f1 = f |+ (ptr,a + sp - (LENGTH ws + 1))`
+  \\ Q.ABBREV_TAC `f1 = f |+ (ptr,a + sp - (ws + 1))`
   \\ `f SUBMAP f1` by ALL_TAC THEN1
    (Q.UNABBREV_TAC `f1` \\ full_simp_tac (srw_ss()) [SUBMAP_DEF,FAPPLY_FUPDATE_THM]
     \\ metis_tac [])
@@ -1976,7 +1982,7 @@ val new_byte_thm = Q.store_thm("new_byte_thm",
    (Q.UNABBREV_TAC `f1` \\ asm_simp_tac (srw_ss()) [bc_ref_inv_def,FDOM_FUPDATE,
       FAPPLY_FUPDATE_THM] \\ full_simp_tac std_ss [el_length_def,Bytes_def,LET_DEF]
     \\ full_simp_tac (srw_ss()) [FLOOKUP_DEF,EVERY2_EQ_EL]
-    \\ rpt strip_tac \\ qexists_tac `ws` \\ fs [])
+    \\ rpt strip_tac \\ qexists_tac `REPLICATE ws 0w` \\ fs [])
   \\ `reachable_refs stack refs n` by
    (fs [reachable_refs_def]
     \\ `ref_edge (refs |+ (ptr,ByteArray fl bs)) = ref_edge refs` by
@@ -2264,13 +2270,15 @@ val word_payload_def = Define `
      (make_header conf 3w l,
       qs, (ys = []) /\ (LENGTH qs = l))) /\
   (word_payload ys l (NumTag b) qs conf =
-     (* header: ...111[11] or ...011[11] here i in ...i[11] must be 1 for GC *)
+     (* header: ...111[11] or ...011[11]
+            here i in ...i[11] must be 1 for GC *)
      (make_header conf (b2w b << 2 || 3w:'a word) (LENGTH qs),
       qs, (ys = []) /\ (LENGTH qs = l) /\
           IS_SOME ((encode_header conf (w2n (b2w b << 2 || 3w:'a word))
                       (LENGTH qs)):'a word option))) /\
   (word_payload ys l (BytesTag fl n) qs conf =
-     (* header: ...101[11] or ...001[11] here i in ...i[11] must be 1 for the GC *)
+     (* header: ...101[11] or ...001[11] (compare-by-contents)
+            here i in ...i[11] must be 1 for the GC *)
      ((make_byte_header conf fl n):'a word,
       qs, (ys = []) /\ (LENGTH qs = l) /\
           let k = if dimindex(:'a) = 32 then 2 else 3 in
@@ -3528,6 +3536,316 @@ val shift_shift_lemma = Q.prove(
   \\ simp_tac bool_ss [Once MULT_COMM]
   \\ rewrite_tac [LT_MULT_LCANCEL,GSYM MULT_ASSOC] \\ fs []);
 
+val write_bytes_APPEND = Q.store_thm("write_bytes_APPEND",
+  `!xs ys vals be.
+      write_bytes vals (xs ++ (ys:'a word list)) be =
+      write_bytes vals xs be ++
+      write_bytes (DROP ((dimindex (:α) DIV 8) * LENGTH xs) vals) ys be`,
+  Induct \\ fs [write_bytes_def,ADD1,RIGHT_ADD_DISTRIB,DROP_DROP_T]);
+
+val bytes_to_word_simp = Q.store_thm("bytes_to_word_simp",
+  `(bytes_to_word k a [] w be = w) /\
+    (bytes_to_word k a (b::bs) w be =
+     if k = 0 then w else set_byte a b (bytes_to_word (k-1) (a+1w) bs w be) be)`,
+  Cases_on `k` \\ fs [bytes_to_word_def]);
+
+val set_byte_sort = Q.store_thm("set_byte_sort",
+  `!n1 n2.
+      set_byte (n2w n1) b1 (set_byte (n2w n2:'a word) b2 w be) be =
+      if n1 = n2 then set_byte (n2w n1) b1 w be else
+      if n1 < dimindex(:α) DIV 8 /\ n2 < dimindex(:α) DIV 8 /\
+         good_dimindex(:α) /\ n2 <> n1
+      then
+        set_byte (n2w n2) b2 (set_byte (n2w n1) b1 w be) be
+      else
+        set_byte (n2w n1) b1 (set_byte (n2w n2) b2 w be) be`,
+  rw [] THEN1
+   (fs [set_byte_def]
+    \\ full_simp_tac (std_ss++wordsLib.WORD_BIT_EQ_ss) [word_slice_alt_def]
+    \\ rw [] \\ eq_tac \\ rw []
+    \\ TRY (`F` by decide_tac)
+    \\ metis_tac [])
+  \\ fs [set_byte_def]
+  \\ full_simp_tac (std_ss++wordsLib.WORD_BIT_EQ_ss) [word_slice_alt_def]
+  \\ rw [] \\ eq_tac \\ rw []
+  \\ TRY (metis_tac [])
+  \\ fs [byte_index_def]
+  \\ fs[labPropsTheory.good_dimindex_def] \\ rfs[dimword_def]
+  \\ Cases_on `be` \\ fs []
+  \\ fs [LESS_4,LESS_8] \\ rfs []);
+
+val (set_byte_sort_dec,set_byte_sort_asc) = let
+  fun cross [] ys = []
+    | cross (x::xs) ys = map (fn y => (x,y)) ys :: cross xs ys
+  val xs = [0,1,2,3,4,5,6,7]
+  val ys = cross xs xs |> Lib.flatten
+  fun f (x,y) =
+    SPECL [numSyntax.term_of_int x,numSyntax.term_of_int y] set_byte_sort
+    |> SIMP_RULE (srw_ss()) [labPropsTheory.good_dimindex_def]
+  val ts1 = filter (fn (x,y) => x < y) ys
+  val ts2 = filter (fn (x,y) => y < x) ys
+  in (LIST_CONJ (map f ts1), LIST_CONJ (map f ts2)) end
+
+val set_byte_eq_ARB = Q.store_thm("set_byte_eq_ARB",
+  `good_dimindex (:α) ==>
+    !x h h'.
+      (set_byte 0w x h be = set_byte 0w x (h':'a word) be <=>
+       set_byte 0w ARB h be = set_byte 0w ARB h' be) /\
+      (set_byte 1w x h be = set_byte 1w x (h':'a word) be <=>
+       set_byte 1w ARB h be = set_byte 1w ARB h' be) /\
+      (set_byte 2w x h be = set_byte 2w x (h':'a word) be <=>
+       set_byte 2w ARB h be = set_byte 2w ARB h' be) /\
+      (set_byte 3w x h be = set_byte 3w x (h':'a word) be <=>
+       set_byte 3w ARB h be = set_byte 3w ARB h' be) /\
+      (set_byte 4w x h be = set_byte 4w x (h':'a word) be <=>
+       set_byte 4w ARB h be = set_byte 4w ARB h' be) /\
+      (set_byte 5w x h be = set_byte 5w x (h':'a word) be <=>
+       set_byte 5w ARB h be = set_byte 5w ARB h' be) /\
+      (set_byte 6w x h be = set_byte 6w x (h':'a word) be <=>
+       set_byte 6w ARB h be = set_byte 6w ARB h' be) /\
+      (set_byte 7w x h be = set_byte 7w x (h':'a word) be <=>
+       set_byte 7w ARB h be = set_byte 7w ARB h' be)`,
+  rw [labPropsTheory.good_dimindex_def]
+  \\ Cases_on `be` \\ fs [set_byte_def,LET_THM,byte_index_def,dimword_def]
+  \\ full_simp_tac (std_ss++wordsLib.WORD_BIT_EQ_ss)
+        [word_slice_alt_def,set_byte_def,LET_THM,dimword_def]);
+
+val bytes_to_word_eq_lemma = Q.store_thm("bytes_to_word_eq_lemma",
+  `good_dimindex (:α) /\ LENGTH bs' = LENGTH bs /\
+    bytes_to_word (dimindex (:α) DIV 8) 0w bs (h:'a word) be =
+    bytes_to_word (dimindex (:α) DIV 8) 0w bs h' be ==>
+    bytes_to_word (dimindex (:α) DIV 8) 0w bs' h be =
+    bytes_to_word (dimindex (:α) DIV 8) 0w bs' h' be`,
+  fs[labPropsTheory.good_dimindex_def] \\ rfs[dimword_def]
+  \\ rw [] \\ rfs [] \\ pop_assum mp_tac
+  \\ `good_dimindex (:α)` by fs[labPropsTheory.good_dimindex_def]
+  \\ Cases_on `bs` \\ Cases_on `bs'` \\ fs [bytes_to_word_simp]
+  \\ assume_tac (UNDISCH set_byte_eq_ARB)
+  \\ pop_assum (fn th => once_rewrite_tac [th]) \\ fs []
+  \\ rpt (rename1 `LENGTH t1 = LENGTH t2`
+    \\ Cases_on `t1` \\ Cases_on `t2` \\ fs [bytes_to_word_simp]
+    \\ NTAC 30 (fs [Once set_byte_sort_dec])
+    \\ assume_tac (UNDISCH set_byte_eq_ARB)
+    \\ pop_assum (fn th => once_rewrite_tac [th])))
+
+val write_bytes_inj_lemma = Q.store_thm("write_bytes_inj_lemma",
+  `good_dimindex(:α) ⇒
+   ∀w1 w2 bs bs'.
+   write_bytes bs w1 be = write_bytes bs (w2:'a word list) be ∧
+   LENGTH w1 = LENGTH w2 ∧
+   LENGTH bs' = LENGTH bs (*∧
+   LENGTH bs ≤ LENGTH (w1:α word list) * (dimindex (:α) DIV 8) *)
+   (* ∧ LENGTH (w1:α word list) ≤ LENGTH bs DIV (dimindex(:α) DIV 8) +1 *)
+   ⇒
+   write_bytes bs' w1 be = write_bytes bs' w2 be`,
+  strip_tac \\ Induct \\ rw[write_bytes_def]
+  >- (
+    `w2 = []` by metis_tac[LENGTH_NIL_SYM]
+    \\ rw[write_bytes_def] )
+  \\ Cases_on`w2` \\ fs[write_bytes_def] \\ rw[]
+  >- (match_mp_tac bytes_to_word_eq_lemma \\ fs [])
+  \\ first_x_assum match_mp_tac
+  \\ rw[] \\ asm_exists_tac \\ simp[]);
+
+(* slow *)
+val set_byte_all_64 = Q.store_thm("set_byte_all_64",
+  `dimindex(:'a) = 64 ⇒
+   set_byte (0w:'a word) b1
+     (set_byte 1w b2
+       (set_byte 2w b3
+         (set_byte 3w b4
+           (set_byte 4w b5
+             (set_byte 5w b6
+               (set_byte 6w b7
+                 (set_byte 7w b8 x be) be) be) be) be) be) be) be
+   =
+   set_byte 0w b1
+     (set_byte 1w b2
+       (set_byte 2w b3
+         (set_byte 3w b4
+           (set_byte 4w b5
+             (set_byte 5w b6
+               (set_byte 6w b7
+                 (set_byte 7w b8 y be) be) be) be) be) be) be) be`,
+  Cases_on`be`
+  \\ rw[set_byte_def,byte_index_def,dimword_def,word_slice_alt_def]
+  \\ srw_tac[wordsLib.WORD_BIT_EQ_ss][]);
+
+val set_byte_all_32 = Q.store_thm("set_byte_all_32",
+  `dimindex(:'a) = 32 ⇒
+   set_byte (0w:'a word) b1
+     (set_byte 1w b2
+       (set_byte 2w b3
+                 (set_byte 3w b8 x be) be) be) be
+   =
+   set_byte 0w b1
+     (set_byte 1w b2
+       (set_byte 2w b3
+                 (set_byte 3w b8 y be) be) be) be`,
+  Cases_on`be`
+  \\ rw[set_byte_def,byte_index_def,dimword_def,word_slice_alt_def]
+  \\ srw_tac[wordsLib.WORD_BIT_EQ_ss][]);
+
+(* slow *)
+val word_of_byte_set_byte_64 = Q.store_thm("word_of_byte_set_byte_64",
+  `dimindex(:'a) = 64 ⇒
+   word_of_byte (w2w w) =
+   set_byte 0w w
+     (set_byte 1w w
+       (set_byte 2w w
+         (set_byte 3w w
+           (set_byte 4w w
+             (set_byte 5w w
+               (set_byte 6w w
+                 (set_byte 7w w (x:'a word) be) be) be) be) be) be) be) be`,
+  rw[word_of_byte_def,set_byte_def,byte_index_def,dimword_def,word_slice_alt_def]
+  \\ srw_tac[wordsLib.WORD_BIT_EQ_ss][]);
+
+val word_of_byte_set_byte_32 = Q.store_thm("word_of_byte_set_byte_32",
+  `dimindex(:'a) = 32 ⇒
+   word_of_byte (w2w w) =
+   set_byte 0w w
+     (set_byte 1w w
+       (set_byte 2w w
+                 (set_byte 3w w (x:'a word) be) be) be) be`,
+  rw[word_of_byte_def,set_byte_def,byte_index_def,dimword_def,word_slice_alt_def]
+  \\ srw_tac[wordsLib.WORD_BIT_EQ_ss][]);
+
+val write_bytes_change_extra = Q.store_thm("write_bytes_change_extra",
+  `∀ws bs be ws'.
+   good_dimindex(:'a) ∧
+   LENGTH ws = LENGTH ws' ∧
+   LENGTH ws < byte_len (:'a) (LENGTH bs)
+   ⇒
+   write_bytes bs (ws:'a word list) be = write_bytes bs ws' be`,
+  Induct \\ rw[write_bytes_def,LENGTH_NIL_SYM]
+  \\ Cases_on`ws'` \\ fs[write_bytes_def]
+  \\ reverse conj_tac
+  >- (
+    first_x_assum match_mp_tac
+    \\ fs[byte_len_def,labPropsTheory.good_dimindex_def]
+    \\ rfs[X_LT_DIV] )
+  \\ fs[labPropsTheory.good_dimindex_def,byte_len_def]
+  \\ Cases_on`bs` \\ rfs[ADD1]
+  \\ qmatch_goalsub_rename_tac`_::bs`
+  \\ Cases_on`bs` \\ rfs[ADD1]
+  \\ qmatch_goalsub_rename_tac`_::_::bs`
+  \\ Cases_on`bs` \\ rfs[ADD1]
+  \\ qmatch_goalsub_rename_tac`_::_::_::bs`
+  \\ Cases_on`bs` \\ rfs[ADD1]
+  \\ qmatch_goalsub_rename_tac`_::_::_::_::bs`
+  \\ Cases_on`bs` \\ rfs[ADD1]
+  \\ TRY (
+    qmatch_goalsub_rename_tac`_::_::_::_::_::bs`
+    \\ Cases_on`bs` \\ rfs[ADD1] )
+  \\ TRY (
+    qmatch_goalsub_rename_tac`_::_::_::_::_::_::bs`
+    \\ Cases_on`bs` \\ rfs[ADD1] )
+  \\ TRY (
+    qmatch_goalsub_rename_tac`_::_::_::_::_::_::_::bs`
+    \\ Cases_on`bs` \\ rfs[ADD1] )
+  \\ TRY (
+    qmatch_goalsub_rename_tac`_::_::_::_::_::_::_::_::bs`
+    \\ Cases_on`bs` \\ rfs[ADD1] )
+  \\ simp[bytes_to_word_simp,set_byte_all_64,set_byte_all_32]);
+
+val byte_len_lemma = Q.store_thm("byte_len_lemma",
+  `good_dimindex(:'a) ∧
+   byte_len (:'a) n = SUC l ⇒
+   n - l * (dimindex (:'a) DIV 8) =
+     if n MOD (dimindex (:'a) DIV 8) = 0
+     then dimindex(:'a) DIV 8
+     else n MOD (dimindex (:'a) DIV 8)`,
+  rw[labPropsTheory.good_dimindex_def,byte_len_def]
+  \\ fs[DIV_EQ_X,MULT_CLAUSES,MOD_EQ_0_DIVISOR] \\ rfs[]
+  \\ fs[MOD_EQ_0_DIVISOR] \\ rfs[]
+  >- ( `4 * l < 4 * d` by decide_tac \\ fs[] )
+  >- (
+    `l = n DIV 4` suffices_by (
+      qspec_then`4`mp_tac DIVISION \\ simp[]
+      \\ disch_then(qspec_then`n`mp_tac)
+      \\ decide_tac )
+    \\ simp[DIV_EQ_X,ADD1,MULT_CLAUSES]
+    \\ `n ≠ 4 * l + 4` suffices_by decide_tac
+    \\ strip_tac \\ fs[]
+    \\ first_x_assum(qspec_then`l+1`mp_tac)
+    \\ simp[] )
+  >- ( `8 * l < 8 * d` by decide_tac \\ fs[] )
+  >- (
+    `l = n DIV 8` suffices_by (
+      qspec_then`8`mp_tac DIVISION \\ simp[]
+      \\ disch_then(qspec_then`n`mp_tac)
+      \\ decide_tac )
+    \\ simp[DIV_EQ_X,ADD1,MULT_CLAUSES]
+    \\ `n ≠ 8 * l + 8` suffices_by decide_tac
+    \\ strip_tac \\ fs[]
+    \\ first_x_assum(qspec_then`l+1`mp_tac)
+    \\ simp[] ));
+
+(*
+val partial_word_of_byte_def = Define`
+  partial_word_of_byte n (w:'a word) be =
+    let w = word_of_byte w in
+    let nb = dimindex(:'a) DIV 8 in
+    let shift = nb - n MOD nb in
+    if shift = nb then w else
+      if be then w << (8 * shift) else w >>> (8 * shift)`;
+
+(* slow *)
+val partial_word_of_byte_bytes_to_word = Q.store_thm("partial_word_of_byte_bytes_to_word",
+  `good_dimindex(:'a) ⇒
+   partial_word_of_byte n ((w2w w):'a word) be =
+     if n MOD (dimindex(:'a) DIV 8) = 0  then
+       word_of_byte (w2w w)
+     else
+     bytes_to_word (dimindex(:'a) DIV 8) 0w (REPLICATE (n MOD (dimindex(:'a) DIV 8)) w) 0w be`,
+  rw[] >- rw[partial_word_of_byte_def]
+  \\ fs[labPropsTheory.good_dimindex_def,partial_word_of_byte_def]
+  >- (
+    qspecl_then[`n`,`4`]mp_tac MOD_LESS
+    \\ impl_tac >- simp[]
+    \\ rewrite_tac[LESS_4]
+    \\ strip_tac \\ fs[REPLICATE_compute,bytes_to_word_simp]
+    \\ rw[word_of_byte_def,set_byte_def,byte_index_def,word_slice_alt_def,dimword_def]
+    \\ srw_tac[wordsLib.WORD_BIT_EQ_ss][] )
+  >- (
+    qspecl_then[`n`,`8`]mp_tac MOD_LESS
+    \\ impl_tac >- simp[]
+    \\ rewrite_tac[LESS_8]
+    \\ strip_tac \\ fs[REPLICATE_compute,bytes_to_word_simp]
+    \\ rw[word_of_byte_def,set_byte_def,byte_index_def,word_slice_alt_def,dimword_def]
+    \\ srw_tac[wordsLib.WORD_BIT_EQ_ss][] ));
+*)
+
+val byte_mask_def = Define`
+  byte_mask (:'a) n be =
+    let nb = dimindex(:'a) DIV 8 in
+    let shift = 8 * ((nb - n MOD nb) MOD nb) in
+    if be then -1w << shift else -1w >>> shift`;
+
+(* slow *)
+val bytes_to_word_byte_mask = Q.store_thm("bytes_to_word_byte_mask",
+  `good_dimindex(:'a) ∧
+   n MOD (dimindex(:'a) DIV 8) ≠ 0 ⇒
+   (word_of_byte ((w2w w):'a word) && byte_mask (:'a) n be) =
+   bytes_to_word (dimindex(:'a) DIV 8) 0w (REPLICATE (n MOD (dimindex(:'a) DIV 8)) w) 0w be`,
+  rw[]
+  \\ fs[labPropsTheory.good_dimindex_def,byte_mask_def]
+  >- (
+    qspecl_then[`n`,`4`]mp_tac MOD_LESS
+    \\ impl_tac >- simp[]
+    \\ rewrite_tac[LESS_4]
+    \\ strip_tac \\ rfs[REPLICATE_compute,bytes_to_word_simp]
+    \\ rw[word_of_byte_def,set_byte_def,byte_index_def,word_slice_alt_def,dimword_def]
+    \\ srw_tac[wordsLib.WORD_BIT_EQ_ss][] )
+  >- (
+    qspecl_then[`n`,`8`]mp_tac MOD_LESS
+    \\ impl_tac >- simp[]
+    \\ rewrite_tac[LESS_8]
+    \\ strip_tac \\ rfs[REPLICATE_compute,bytes_to_word_simp]
+    \\ rw[word_of_byte_def,set_byte_def,byte_index_def,word_slice_alt_def,dimword_def]
+    \\ srw_tac[wordsLib.WORD_BIT_EQ_ss][] ));
+
 val memory_rel_RefByte = Q.store_thm("memory_rel_RefByte",
  `memory_rel c be refs sp st m dm vars ∧
    new ∉ FDOM refs ∧ byte_len (:'a) n < sp ∧
@@ -3537,11 +3855,10 @@ val memory_rel_RefByte = Q.store_thm("memory_rel_RefByte",
    ∃eoh curr m1.
      FLOOKUP st EndOfHeap = SOME (Word eoh) ∧
      FLOOKUP st CurrHeap = SOME (Word curr) ∧
-     (let w' = eoh − bytes_in_word * (n2w (byte_len (:'a) n + 1)) :'a word
-      in
-        store_list w' (Word (make_byte_header c fl n)::
-          REPLICATE (byte_len (:'a) n)
-            (Word (word_of_byte (w2w w)))) m dm = SOME m1 ∧
+     (let w' = eoh − bytes_in_word * (n2w (byte_len (:'a) n + 1)) :'a word in
+      let ws = REPLICATE (byte_len (:'a) n) (Word (word_of_byte (w2w w))) in
+      let ws = LUPDATE (Word (byte_mask (:'a) n be && word_of_byte (w2w w))) (byte_len (:'a) n - 1) ws in
+        store_list w' (Word (make_byte_header c fl n)::ws) m dm = SOME m1 ∧
         memory_rel c be (refs |+ (new,ByteArray fl (REPLICATE n w)))
           (sp − (byte_len (:'a) n + 1)) (st |+ (EndOfHeap,Word w')) m1 dm
           ((RefPtr new,make_ptr c (w' − curr) 0w (byte_len (:'a) n))::vars))`,
@@ -3551,7 +3868,7 @@ val memory_rel_RefByte = Q.store_thm("memory_rel_RefByte",
   \\ fs [memory_rel_def,PULL_EXISTS] \\ rw []
   \\ fs [word_ml_inv_def,PULL_EXISTS] \\ clean_tac
   \\ drule (GEN_ALL new_byte_thm)
-  \\ disch_then (qspecl_then [`REPLICATE (byte_len (:'a) n) (word_of_byte (w2w w))`,
+  \\ disch_then (qspecl_then [`(byte_len (:'a) n)`,
         `new`,`fl`,`REPLICATE n w`] mp_tac)
   \\ fs [LENGTH_REPLICATE]
   \\ impl_tac THEN1
@@ -3606,7 +3923,31 @@ val memory_rel_RefByte = Q.store_thm("memory_rel_RefByte",
   \\ fs [GSYM bytes_in_word_mul_eq_shift,write_bytes_REPLICATE]
   \\ qpat_abbrev_tac `ws = Word (make_byte_header c fl n)::_`
   \\ qpat_abbrev_tac `ws1 = Word (make_byte_header c fl n)::_`
-  \\ `ws1 = ws` by (unabbrev_all_tac \\ fs [map_replicate] \\ NO_TAC)
+  \\ `ws1 = ws` by (
+    unabbrev_all_tac \\ fs [map_replicate] \\
+    Cases_on`byte_len (:'a) n` \\ fs[]
+    >- ( fs[byte_len_def,REPLICATE,LUPDATE_def,write_bytes_def] )
+    \\ rename1`REPLICATE (SUC l)`
+    \\ simp[REPLICATE_SNOC,LUPDATE_APPEND2,LUPDATE_def,write_bytes_APPEND]
+    \\ simp[APPEND_EQ_APPEND] \\ disj1_tac \\ qexists_tac`[]` \\ simp[]
+    \\ conj_tac
+    >- (
+      once_rewrite_tac[GSYM map_replicate]
+      \\ AP_TERM_TAC
+      \\ drule(GSYM write_bytes_REPLICATE)
+      \\ disch_then(qspecl_then[`l`,`n`]SUBST_ALL_TAC)
+      \\ match_mp_tac write_bytes_change_extra
+      \\ simp[] )
+    \\ simp[write_bytes_def]
+    \\ simp[DROP_REPLICATE]
+    \\ simp[byte_len_lemma]
+    \\ IF_CASES_TAC
+    >- (
+      rw[byte_mask_def]
+      \\ fs[labPropsTheory.good_dimindex_def,REPLICATE_compute,bytes_to_word_simp]
+      \\ simp[word_of_byte_set_byte_32,word_of_byte_set_byte_64] )
+    \\ simp[bytes_to_word_byte_mask]
+    \\ NO_TAC)
   \\ rveq \\ fs []
   \\ simp_tac (std_ss++helperLib.sep_cond_ss) [cond_STAR,GSYM CONJ_ASSOC]
   \\ fs [GSYM PULL_EXISTS] \\ fs [CONJ_ASSOC]
@@ -4044,17 +4385,6 @@ val LESS_LENGTH_IMP = Q.prove(
   Induct \\ fs [] \\ Cases_on `n` \\ fs [LENGTH_NIL] \\ rw []
   \\ res_tac \\ clean_tac \\ qexists_tac `h::ys` \\ fs []);
 
-val write_bytes_APPEND = Q.store_thm("write_bytes_APPEND",
-  `!xs ys vals be.
-      write_bytes vals (xs ++ (ys:'a word list)) be =
-      write_bytes vals xs be ++
-      write_bytes (DROP ((dimindex (:α) DIV 8) * LENGTH xs) vals) ys be`,
-  Induct \\ fs [write_bytes_def,ADD1,RIGHT_ADD_DISTRIB,DROP_DROP_T]);
-
-val LESS_4 = DECIDE ``i < 4 <=> (i = 0) \/ (i = 1) \/ (i = 2) \/ (i = 3n)``
-val LESS_8 = DECIDE ``i < 8 <=> (i = 0) \/ (i = 1) \/ (i = 2) \/ (i = 3n) \/
-                                (i = 4) \/ (i = 5) \/ (i = 6) \/ (i = 7)``
-
 val expand_num =
   DECIDE ``4 = SUC 3 /\ 3 = SUC 2 /\ 2 = SUC 1 /\ 1 = SUC 0 /\
            5 = SUC 4 /\ 6 = SUC 5 /\ 7 = SUC 6 /\ 8 = SUC 7``
@@ -4267,110 +4597,6 @@ val write_bytes_same = Q.store_thm("write_bytes_same",
   \\ qpat_abbrev_tac`bw= _ DIV _`
   \\ first_x_assum(qspec_then`n+bw`mp_tac)
   \\ simp[EL_DROP]);
-
-val bytes_to_word_simp = Q.store_thm("bytes_to_word_simp",
-  `(bytes_to_word k a [] w be = w) /\
-    (bytes_to_word k a (b::bs) w be =
-     if k = 0 then w else set_byte a b (bytes_to_word (k-1) (a+1w) bs w be) be)`,
-  Cases_on `k` \\ fs [bytes_to_word_def]);
-
-val set_byte_sort = Q.store_thm("set_byte_sort",
-  `!n1 n2.
-      set_byte (n2w n1) b1 (set_byte (n2w n2:'a word) b2 w be) be =
-      if n1 = n2 then set_byte (n2w n1) b1 w be else
-      if n1 < dimindex(:α) DIV 8 /\ n2 < dimindex(:α) DIV 8 /\
-         good_dimindex(:α) /\ n2 <> n1
-      then
-        set_byte (n2w n2) b2 (set_byte (n2w n1) b1 w be) be
-      else
-        set_byte (n2w n1) b1 (set_byte (n2w n2) b2 w be) be`,
-  rw [] THEN1
-   (fs [set_byte_def]
-    \\ full_simp_tac (std_ss++wordsLib.WORD_BIT_EQ_ss) [word_slice_alt_def]
-    \\ rw [] \\ eq_tac \\ rw []
-    \\ TRY (`F` by decide_tac)
-    \\ metis_tac [])
-  \\ fs [set_byte_def]
-  \\ full_simp_tac (std_ss++wordsLib.WORD_BIT_EQ_ss) [word_slice_alt_def]
-  \\ rw [] \\ eq_tac \\ rw []
-  \\ TRY (metis_tac [])
-  \\ fs [byte_index_def]
-  \\ fs[labPropsTheory.good_dimindex_def] \\ rfs[dimword_def]
-  \\ Cases_on `be` \\ fs []
-  \\ fs [LESS_4,LESS_8] \\ rfs []);
-
-val (set_byte_sort_dec,set_byte_sort_asc) = let
-  fun cross [] ys = []
-    | cross (x::xs) ys = map (fn y => (x,y)) ys :: cross xs ys
-  val xs = [0,1,2,3,4,5,6,7]
-  val ys = cross xs xs |> Lib.flatten
-  fun f (x,y) =
-    SPECL [numSyntax.term_of_int x,numSyntax.term_of_int y] set_byte_sort
-    |> SIMP_RULE (srw_ss()) [labPropsTheory.good_dimindex_def]
-  val ts1 = filter (fn (x,y) => x < y) ys
-  val ts2 = filter (fn (x,y) => y < x) ys
-  in (LIST_CONJ (map f ts1), LIST_CONJ (map f ts2)) end
-
-val set_byte_eq_ARB = Q.store_thm("set_byte_eq_ARB",
-  `good_dimindex (:α) ==>
-    !x h h'.
-      (set_byte 0w x h be = set_byte 0w x (h':'a word) be <=>
-       set_byte 0w ARB h be = set_byte 0w ARB h' be) /\
-      (set_byte 1w x h be = set_byte 1w x (h':'a word) be <=>
-       set_byte 1w ARB h be = set_byte 1w ARB h' be) /\
-      (set_byte 2w x h be = set_byte 2w x (h':'a word) be <=>
-       set_byte 2w ARB h be = set_byte 2w ARB h' be) /\
-      (set_byte 3w x h be = set_byte 3w x (h':'a word) be <=>
-       set_byte 3w ARB h be = set_byte 3w ARB h' be) /\
-      (set_byte 4w x h be = set_byte 4w x (h':'a word) be <=>
-       set_byte 4w ARB h be = set_byte 4w ARB h' be) /\
-      (set_byte 5w x h be = set_byte 5w x (h':'a word) be <=>
-       set_byte 5w ARB h be = set_byte 5w ARB h' be) /\
-      (set_byte 6w x h be = set_byte 6w x (h':'a word) be <=>
-       set_byte 6w ARB h be = set_byte 6w ARB h' be) /\
-      (set_byte 7w x h be = set_byte 7w x (h':'a word) be <=>
-       set_byte 7w ARB h be = set_byte 7w ARB h' be)`,
-  rw [labPropsTheory.good_dimindex_def]
-  \\ Cases_on `be` \\ fs [set_byte_def,LET_THM,byte_index_def,dimword_def]
-  \\ full_simp_tac (std_ss++wordsLib.WORD_BIT_EQ_ss)
-        [word_slice_alt_def,set_byte_def,LET_THM,dimword_def]);
-
-val bytes_to_word_eq_lemma = Q.store_thm("bytes_to_word_eq_lemma",
-  `good_dimindex (:α) /\ LENGTH bs' = LENGTH bs /\
-    bytes_to_word (dimindex (:α) DIV 8) 0w bs (h:'a word) be =
-    bytes_to_word (dimindex (:α) DIV 8) 0w bs h' be ==>
-    bytes_to_word (dimindex (:α) DIV 8) 0w bs' h be =
-    bytes_to_word (dimindex (:α) DIV 8) 0w bs' h' be`,
-  fs[labPropsTheory.good_dimindex_def] \\ rfs[dimword_def]
-  \\ rw [] \\ rfs [] \\ pop_assum mp_tac
-  \\ `good_dimindex (:α)` by fs[labPropsTheory.good_dimindex_def]
-  \\ Cases_on `bs` \\ Cases_on `bs'` \\ fs [bytes_to_word_simp]
-  \\ assume_tac (UNDISCH set_byte_eq_ARB)
-  \\ pop_assum (fn th => once_rewrite_tac [th]) \\ fs []
-  \\ rpt (rename1 `LENGTH t1 = LENGTH t2`
-    \\ Cases_on `t1` \\ Cases_on `t2` \\ fs [bytes_to_word_simp]
-    \\ NTAC 30 (fs [Once set_byte_sort_dec])
-    \\ assume_tac (UNDISCH set_byte_eq_ARB)
-    \\ pop_assum (fn th => once_rewrite_tac [th])))
-
-val write_bytes_inj_lemma = Q.store_thm("write_bytes_inj_lemma",
-  `good_dimindex(:α) ⇒
-   ∀w1 w2 bs bs'.
-   write_bytes bs w1 be = write_bytes bs (w2:'a word list) be ∧
-   LENGTH w1 = LENGTH w2 ∧
-   LENGTH bs' = LENGTH bs (*∧
-   LENGTH bs ≤ LENGTH (w1:α word list) * (dimindex (:α) DIV 8) *)
-   (* ∧ LENGTH (w1:α word list) ≤ LENGTH bs DIV (dimindex(:α) DIV 8) +1 *)
-   ⇒
-   write_bytes bs' w1 be = write_bytes bs' w2 be`,
-  strip_tac \\ Induct \\ rw[write_bytes_def]
-  >- (
-    `w2 = []` by metis_tac[LENGTH_NIL_SYM]
-    \\ rw[write_bytes_def] )
-  \\ Cases_on`w2` \\ fs[write_bytes_def] \\ rw[]
-  >- (match_mp_tac bytes_to_word_eq_lemma \\ fs [])
-  \\ first_x_assum match_mp_tac
-  \\ rw[] \\ asm_exists_tac \\ simp[]);
 
 val set_byte_change_a = Q.store_thm("set_byte_change_a",
   `w2n (a:α word) MOD (dimindex(:α) DIV 8) = w2n a' MOD (dimindex(:α) DIV 8) ⇒
@@ -4613,7 +4839,9 @@ val memory_rel_ByteArray_IMP = Q.store_thm("memory_rel_ByteArray_IMP",
   `memory_rel c be refs sp st m dm ((RefPtr p,v:'a word_loc)::vars) /\
    FLOOKUP refs p = SOME (ByteArray fl vals) /\ good_dimindex (:'a) ==>
    ?w a x l.
-     v = Word w /\ w ' 0 /\ ~(word_bit 3 x) /\ (word_bit 4 x ⇔ ¬fl) /\ word_bit 2 x /\
+     v = Word w /\ w ' 0 /\
+     make_byte_header c fl (LENGTH vals) = x /\
+     ~(word_bit 3 x) /\ (word_bit 4 x ⇔ ¬fl) /\ word_bit 2 x /\
      get_real_addr c st w = SOME a /\ m a = Word x /\ a IN dm /\
      (!i. i < LENGTH vals ==>
           mem_load_byte_aux m dm be (a + bytes_in_word + n2w i) =
@@ -4631,6 +4859,7 @@ val memory_rel_ByteArray_IMP = Q.store_thm("memory_rel_ByteArray_IMP",
        LENGTH vals + 7 < 2 ** (dimindex (:'a) - 3) /\
        (x >>> (dimindex (:'a) - c.len_size - 3) = n2w (LENGTH vals + 7))`,
   CONV_TAC(RAND_CONV(REWRITE_CONV[GSYM hide_memory_rel_def]))
+  \\ qpat_abbrev_tac`P = $= (make_byte_header _ _ _)`
   \\ fs [memory_rel_def,word_ml_inv_def,PULL_EXISTS,
          bc_stack_ref_inv_def,v_inv_def,word_addr_def]
   \\ rpt strip_tac
@@ -4654,6 +4883,7 @@ val memory_rel_ByteArray_IMP = Q.store_thm("memory_rel_ByteArray_IMP",
          word_payload_def,word_list_def,Bytes_def]
   \\ full_simp_tac (std_ss++sep_cond_ss) [cond_STAR]
   \\ imp_res_tac EVERY2_LENGTH \\ SEP_R_TAC \\ fs [get_addr_0]
+  \\ simp[Abbr`P`]
   \\ conj_asm1_tac
   THEN1 (fs [make_byte_header_def,word_bit_def,word_or_def,fcpTheory.FCP_BETA]
     \\ fs [labPropsTheory.good_dimindex_def]
@@ -4712,7 +4942,7 @@ val memory_rel_ByteArray_IMP = Q.store_thm("memory_rel_ByteArray_IMP",
       \\ qpat_x_assum `_ = _` (fn th => simp_tac std_ss [Once th])
       \\ Cases_on `curr` \\ fs [word_add_n2w,word_mul_n2w] \\ NO_TAC)
     \\ fs []
-    \\ `i DIV 2 ** k < LENGTH ws` by
+    \\ `i DIV 2 ** k < ws` by
         (fs [DIV_LT_X,RIGHT_ADD_DISTRIB]
          \\ `0n < 2 ** k` by fs []
          \\ rpt_drule DIVISION
@@ -4722,8 +4952,8 @@ val memory_rel_ByteArray_IMP = Q.store_thm("memory_rel_ByteArray_IMP",
           n2w (heap_length ha) * n2w (2 ** k) IN dm) /\
         m (curr + n2w (i DIV 2 ** k * 2 ** k) + n2w (2 ** k) +
           n2w (heap_length ha) * n2w (2 ** k)) =
-        (EL (i DIV 2 ** k) (MAP Word (write_bytes vals ws be)))` by
-     (`i DIV 2 ** k < LENGTH (MAP Word (write_bytes vals ws be))` by
+        (EL (i DIV 2 ** k) (MAP Word (write_bytes vals (REPLICATE ws 0w) be)))` by
+     (`i DIV 2 ** k < LENGTH (MAP Word (write_bytes vals (REPLICATE ws 0w) be))` by
                 (fs [] \\ decide_tac)
       \\ drule LESS_LENGTH_IMP \\ strip_tac \\ clean_tac
       \\ fs [word_list_def,word_list_APPEND,bytes_in_word_def,word_mul_n2w]
@@ -4732,11 +4962,13 @@ val memory_rel_ByteArray_IMP = Q.store_thm("memory_rel_ByteArray_IMP",
       \\ simp_tac std_ss [GSYM APPEND_ASSOC,APPEND]
       \\ fs [EL_LENGTH_APPEND])
     \\ fs [EL_MAP,LENGTH_write_bytes]
+    \\ `i DIV 2 ** k < LENGTH (REPLICATE ws 0w)` by simp[]
     \\ drule LESS_LENGTH_IMP \\ strip_tac \\ clean_tac
     \\ fs [write_bytes_APPEND]
     \\ `i DIV 2 ** k = LENGTH (write_bytes vals ys be)` by
           metis_tac [LENGTH_write_bytes]
-    \\ full_simp_tac std_ss [EL_LENGTH_APPEND,NULL_DEF,write_bytes_def,LET_DEF]
+    \\ asm_simp_tac std_ss [write_bytes_def,LET_DEF,GSYM APPEND_ASSOC,APPEND]
+    \\ asm_simp_tac std_ss [EL_LENGTH_APPEND,NULL_DEF,HD]
     \\ fs [] \\ pop_assum (fn th => fs [GSYM th]) \\ fs []
     \\ `EL i vals =
         EL (i MOD 2 ** k) (DROP (i DIV 2 ** k * 2 ** k) vals)` by
@@ -4762,15 +4994,18 @@ val memory_rel_ByteArray_IMP = Q.store_thm("memory_rel_ByteArray_IMP",
     \\ fs[wordSemTheory.mem_load_byte_aux_def]
     \\ Cases_on`m (byte_align ad)` \\ fs[]
     \\ qmatch_asmsub_abbrev_tac`ha ++ bytes ::hb`
-    \\ `bytes = Bytes be fl vals ws` by simp[Abbr`bytes`,Bytes_def]
+    \\ `bytes = Bytes be fl vals (REPLICATE ws 0w)` by simp[Abbr`bytes`,Bytes_def]
     \\ qunabbrev_tac`bytes` \\ fs[]
     \\ simp[theWord_def]
     \\ rfs[]
     \\ first_x_assum(qspecl_then[`i`,`ha`]mp_tac o CONV_RULE(RESORT_FORALL_CONV(sort_vars["i'","ha'"])))
     \\ simp[]
     \\ pop_assum (assume_tac o SYM)
-    \\ disch_then drule
+    \\ simp[]
     \\ pop_assum (assume_tac o SYM)
+    \\ disch_then(qspec_then`REPLICATE ws 0w`mp_tac) \\ simp[]
+    \\ disch_then(qspec_then`vals`mp_tac) \\ simp[]
+    \\ disch_then(qspec_then`be`mp_tac) \\ simp[]
     \\ disch_then(qspec_then`w`mp_tac)
     \\ simp[hide_heap_in_memory_store_def]
     \\ strip_tac
@@ -4794,7 +5029,7 @@ val memory_rel_ByteArray_IMP = Q.store_thm("memory_rel_ByteArray_IMP",
       \\ fs[el_length_def]
       \\ fs[integerTheory.EQ_ADDL,el_length_def,Bytes_def])
     \\ fs[] \\ clean_tac
-    \\ `write_bytes vals ws be = write_bytes vals ws' be`
+    \\ `write_bytes vals (REPLICATE (LENGTH ws') 0w) be = write_bytes vals ws' be`
     by (
       Q.ISPEC_THEN`Word`match_mp_tac INJ_MAP_EQ
       \\ simp[INJ_DEF] )
@@ -4881,7 +5116,7 @@ val memory_rel_RefPtr_IMP = Q.store_thm("memory_rel_RefPtr_IMP",
   `memory_rel c be refs sp st m dm ((RefPtr p,v:'a word_loc)::vars) /\
     good_dimindex (:'a) ==>
     ?w a x.
-      v = Word w /\ w ' 0 /\ (word_bit 2 x <=> word_bit 4 x) /\
+      v = Word w /\ w ' 0 /\ (word_bit 4 x ==> word_bit 2 x) /\
       (word_bit 3 x <=> ~word_bit 2 x) /\
       get_real_addr c st w = SOME a /\ m a = Word x /\ a IN dm`,
   strip_tac \\ drule memory_rel_RefPtr_IMP_lemma \\ strip_tac
@@ -5830,8 +6065,8 @@ val memory_rel_pointer_eq_size = Q.store_thm("memory_rel_pointer_eq_size",
 
 val do_eq_list_F_IMP_MEM = prove(
   ``!l l'.
-      do_eq_list l l' = Eq_val F /\ LENGTH l' = LENGTH l ==>
-      ?i. i < LENGTH l /\ do_eq (EL i l) (EL i l') = Eq_val F``,
+      do_eq_list refs l l' = Eq_val F /\ LENGTH l' = LENGTH l ==>
+      ?i. i < LENGTH l /\ do_eq refs (EL i l) (EL i l') = Eq_val F``,
   Induct \\ Cases_on `l'` \\ fs [] \\ rpt strip_tac
   \\ every_case_tac \\ fs [] \\ res_tac
   THEN1 (qexists_tac `SUC i` \\ fs [])
@@ -5846,10 +6081,12 @@ val memory_rel_rotate3 = prove(
 val memory_rel_pointer_eq = Q.store_thm("memory_rel_pointer_eq",
   `∀v1 v2 w b.
    good_dimindex (:'a) ∧
-   do_eq v1 v2 = Eq_val b /\
+   do_eq refs v1 v2 = Eq_val b /\
    memory_rel c be refs sp st m dm ((v1,(w:'a word_loc))::(v2,w)::vars) ==> b`,
   ho_match_mp_tac v_ind \\ rw[] \\ Cases_on`v2` \\ fs[] \\ rveq
-  \\ TRY (rpt_drule memory_rel_RefPtr_EQ \\ strip_tac \\ fs [] \\ rfs [] \\ NO_TAC)
+  \\ TRY (
+    rpt_drule memory_rel_RefPtr_EQ \\ strip_tac \\ fs []
+    \\ every_case_tac \\ fs[] \\ rfs[] \\ NO_TAC)
   >- (
     rpt_drule memory_rel_Number_cmp \\ rw[]
     \\ fs[WORD_LESS_REFL]
@@ -6199,7 +6436,7 @@ val memory_rel_limit = Q.store_thm("memory_rel_limit",
 
 val memory_rel_ptr_eq = Q.store_thm("memory_rel_ptr_eq",
   `memory_rel c be refs sp st m dm ((v1,x1)::(v2,x1:'a word_loc)::vars) /\
-   do_eq v1 v2 = Eq_val b /\
+   do_eq refs v1 v2 = Eq_val b /\
    good_dimindex (:'a) ==> b`,
   rw [] \\ CCONTR_TAC \\ fs [] \\ rveq
   \\ imp_res_tac memory_rel_pointer_eq);
@@ -6218,14 +6455,19 @@ val memory_rel_Block_Block_small_eq = prove(
 
 val memory_rel_simple_eq = Q.store_thm("memory_rel_simple_eq",
   `memory_rel c be refs sp st m dm ((v1,x1)::(v2,x2)::vars) /\
-   do_eq v1 v2 = Eq_val b /\
+   do_eq refs v1 v2 = Eq_val b /\
    good_dimindex (:'a) ==>
    ?w1 w2:'a word.
      x1 = Word w1 /\ x2 = Word w2 /\
      (~word_bit 0 w1 \/ ~word_bit 0 w2 ==>
      (w1 = w2) = b)`,
   Cases_on `v1` \\ Cases_on `v2` \\ fs [do_eq_def] \\ rpt strip_tac
-  \\ TRY (drule memory_rel_RefPtr_EQ \\ fs [] \\ rw [] \\ fs [] \\ NO_TAC)
+  \\ TRY (
+    drule memory_rel_RefPtr_EQ \\ fs [] \\ rw []
+    \\ imp_res_tac memory_rel_RefPtr_IMP
+    \\ imp_res_tac memory_rel_tl
+    \\ imp_res_tac memory_rel_RefPtr_IMP
+    \\ fs[word_bit_def] \\ NO_TAC)
   THEN1
    (rpt_drule memory_rel_Number_cmp \\ strip_tac \\ fs []
     \\ reverse (Cases_on `word_bit 0 w1`) \\ fs []
@@ -6296,8 +6538,10 @@ val word_eq_def = tDefine "word_eq" `
                  (a1+bytes_in_word) (a2+bytes_in_word) else
            if ~(h1 = h2) then SOME (0w,l) else
            if ~(word_bit 2 h1) (* is array *) then SOME (0w,l) else
-           if ~(word_bit 3 h1) (* is byte array *) then SOME (0w,l) else
-             (* must be a bignum or word64 *)
+           if ~(word_bit 3 h1) /\ word_bit 4 h1 (* is cmp-by-pointer byte array *) then
+             SOME (0w,l)
+           else
+             (* must be a bignum or word64 or cmp-by-contents byte array *)
             (if l <= w2n (decode_length c h1) then NONE else
              case word_cmp_loop (decode_length c h1)
                (a1 + bytes_in_word * (decode_length c h1))
@@ -6450,20 +6694,20 @@ val memory_rel_Loc = store_thm("memory_rel_Loc",
   \\ every_case_tac \\ fs [] \\ rveq \\ fs [word_addr_def]);
 
 val word_eq_thm = store_thm("word_eq_thm",
-  ``(!v1 v2 l b w1 w2.
+  ``(!refs v1 v2 l b w1 w2.
        memory_rel c be refs sp st m dm
           ((v1,Word w1)::(v2,Word w2:'a word_loc)::vars) /\
-       do_eq v1 v2 = Eq_val b /\
+       do_eq refs v1 v2 = Eq_val b /\
        vb_size v1 * dimword (:'a) < l /\ good_dimindex (:'a) ==>
        ?res l1. word_eq c st dm m l w1 w2 = SOME (res,l1) /\
                 (b <=> (res = 1w)) /\
                 l <= l1 + vb_size v1 * dimword (:'a)) /\
-    (!v1 v2 l b w1 w2 t1 t2.
+    (!refs v1 v2 l b w1 w2 t1 t2.
        memory_rel c be refs sp st m dm
           (eq_explode w1 m dm v1 ++ eq_explode w2 m dm v2 ++ vars) /\
        LENGTH v2 = LENGTH v1 /\ LENGTH v1 < dimword (:'a) /\
        eq_assum w1 m dm v1 /\ eq_assum w2 m dm v2 /\
-       do_eq_list v1 v2 = Eq_val b /\
+       do_eq_list refs v1 v2 = Eq_val b /\
        (LENGTH v1 + SUM (MAP vb_size v1)) * dimword (:'a) < l /\
        good_dimindex (:'a) ==>
        ?res l1. word_eq_list c st dm m l (n2w (LENGTH v1)) w1 w2 = SOME (res,l1) /\
@@ -6539,12 +6783,63 @@ val word_eq_thm = store_thm("word_eq_thm",
     \\ strip_tac
     \\ once_rewrite_tac [word_eq_def]
     \\ IF_CASES_TAC \\ fs []
+    >- ( every_case_tac \\ fs[] )
     \\ drule memory_rel_RefPtr_IMP \\ fs []
     \\ drule memory_rel_tail \\ strip_tac
     \\ drule memory_rel_RefPtr_IMP \\ fs []
     \\ rpt strip_tac \\ fs [word_bit,word_header_def]
     \\ IF_CASES_TAC \\ fs []
-    \\ IF_CASES_TAC \\ fs [] \\ fs [])
+    \\ IF_CASES_TAC \\ fs [] \\ fs []
+    >- (
+      every_case_tac \\  fs[]
+      \\ drule (GEN_ALL memory_rel_ByteArray_IMP)
+      \\ qhdtm_x_assum`memory_rel`kall_tac
+      \\ drule (GEN_ALL memory_rel_ByteArray_IMP)
+      \\ simp[] \\ strip_tac \\ fs[]
+      \\ simp[] \\ strip_tac \\ fs[]
+      \\ clean_tac \\ strip_tac \\  fs[] )
+    \\ IF_CASES_TAC \\ fs [] \\ fs []
+    >- (
+      every_case_tac \\  fs[]
+      \\ drule (GEN_ALL memory_rel_ByteArray_IMP)
+      \\ qhdtm_x_assum`memory_rel`kall_tac
+      \\ drule (GEN_ALL memory_rel_ByteArray_IMP)
+      \\ simp[] \\ strip_tac \\ fs[]
+      \\ simp[] \\ strip_tac \\ fs[]
+      \\ clean_tac \\ strip_tac \\  fs[] )
+    \\ IF_CASES_TAC \\ fs [] \\ fs []
+    >- (
+      every_case_tac \\  fs[]
+      \\ drule (GEN_ALL memory_rel_ByteArray_IMP)
+      \\ qhdtm_x_assum`memory_rel`kall_tac
+      \\ drule (GEN_ALL memory_rel_ByteArray_IMP)
+      \\ simp[] \\ strip_tac \\ fs[]
+      \\ simp[] \\ strip_tac \\ fs[]
+      \\ clean_tac \\ strip_tac \\  fs[] )
+    \\ clean_tac \\ fs[]
+    \\ fs[vb_size_def]
+    \\ imp_res_tac memory_rel_RefPtr_IMP_lemma \\ fs[]
+    \\ `∃bs1 bs2.
+          FLOOKUP refs n1 = SOME (ByteArray T bs1) ∧
+          FLOOKUP refs n2 = SOME (ByteArray T bs2)`
+    by (
+      every_case_tac \\ fs[]
+      \\ drule (GEN_ALL memory_rel_ValueArray_IMP) \\ fs[]
+      \\ drule (GEN_ALL memory_rel_ByteArray_IMP) \\ fs[]
+      \\ qhdtm_x_assum`memory_rel`kall_tac
+      \\ drule (GEN_ALL memory_rel_ValueArray_IMP) \\ fs[]
+      \\ drule (GEN_ALL memory_rel_ByteArray_IMP) \\ fs[]
+      \\ strip_tac \\ fs[])
+    \\ fs[] \\ clean_tac \\ fs[] \\ clean_tac
+    \\ drule (GEN_ALL memory_rel_ByteArray_IMP) \\ fs[]
+    \\ qhdtm_x_assum`memory_rel`kall_tac
+    \\ drule (GEN_ALL memory_rel_ByteArray_IMP) \\ fs[]
+    \\ strip_tac \\ fs[] \\ strip_tac \\ fs[]
+    \\ simp[GSYM CONJ_ASSOC,RIGHT_EXISTS_AND_THM]
+    (*
+    \\ `decode_length c (make_byte_header c T (LENGTH bs1)) = (n2w(LENGTH bs1):'a word)`
+    *)
+    \\ cheat)
   THEN1 (* do_eq Blocks *)
    (rpt gen_tac \\ strip_tac \\ rpt gen_tac
     \\ IF_CASES_TAC THEN1
@@ -6625,7 +6920,7 @@ val word_eq_thm = store_thm("word_eq_thm",
   \\ strip_tac
   \\ once_rewrite_tac [word_eq_def]
   \\ fs [ADD1,word_add_n2w]
-  \\ Cases_on `do_eq v1 v2` \\ fs []
+  \\ Cases_on `do_eq refs v1 v2` \\ fs []
   \\ `?c1. m w1 = Word c1` by
    (Cases_on `m w1` \\ fs [] \\ imp_res_tac memory_rel_Loc
     \\ rveq \\ fs [do_eq_def])
@@ -6660,7 +6955,7 @@ val word_eq_thm = store_thm("word_eq_thm",
 val word_eq_thm = store_thm("word_eq_thm",
   ``memory_rel c be refs sp st m dm
       ((v1,Word w1)::(v2,Word w2:'a word_loc)::vars) /\
-    do_eq v1 v2 = Eq_val b /\ good_dimindex (:'a) ==>
+    do_eq refs v1 v2 = Eq_val b /\ good_dimindex (:'a) ==>
     ?res l1.
        word_eq c st dm m (MustTerminate_limit (:'a) - 1) w1 w2 = SOME (res,l1) /\
        (b <=> (res = 1w))``,
